\documentclass[]{article}

\usepackage{amsmath}

%opening
\title{}
\author{}

\begin{document}

\maketitle

\begin{abstract}
$$ V = \left \{ v_{1}, v_{2}, v_{3}, v_{4} \right \} $$
$$ E = \left \{ e_{1}, e_{2}, e_{3}		   \right \} $$
$$ G = \left \{ V, E \right \} $$

$$ D = 
\begin{bmatrix}
	3  &  &  & \\
	&  1  &  & \\
	&  &  1  & \\
	&  &  &  1
\end{bmatrix}
$$

$$ A = 
\begin{bmatrix}
	0 & 1 & 1 & 1 \\
	1 & 0 &   &	  \\
	1 &   & 0 &	  \\
	1 &   &   & 0
\end{bmatrix}
$$

$$ L = D - A = 
\begin{bmatrix}
	3 & -1 & -1 & -1 \\
	-1&  1 &    &	 \\
	-1&    &  1 &	 \\
	-1&    &    &  1
\end{bmatrix}
$$

$$ \left | \lambda I - L \right | = 0 $$
$$ L \overrightarrow{u} = \lambda \overrightarrow{u} $$

$$
L = 
U \Lambda U^{T}
= 
\sum_{1}^{N}
\lambda _{k}
\overrightarrow{u_{k}}
\cdot
\overrightarrow{u_{k}}^{T}
$$



$$ \forall \overrightarrow{s} \in R^{N} $$
$$
p_{k} = 
\left | \overrightarrow{s} \right | \cos \theta_{k}
= 
\frac
{\overrightarrow{u_{k}}^{T} \cdot \overrightarrow{s}}
{\left | \overrightarrow{u_{k}}^{T} \right |}
= 
\overrightarrow{u_{k}}^{T} \cdot \overrightarrow{s}
$$

$$ \overrightarrow{p} = U^{T} \overrightarrow{s} $$
$$ \overrightarrow{s} = U \overrightarrow{p} $$

$$
TV \left ( \overrightarrow{s} \right )
= 
\overrightarrow{s}^{T} L \overrightarrow{s}
= 
\overrightarrow{s}^{T} U \Lambda U^{T} \overrightarrow{s}
$$

$$
= 
\left ( U^{T} \overrightarrow{s} \right ) ^{T}
\Lambda
\left ( U^{T} \overrightarrow{s} \right )
= 
\overrightarrow{p}^{T}
\Lambda
\overrightarrow{p}
= 
\sum_{1}^{N}
p_{k}^{2} \lambda_{k} \ge 0
$$

$$
E \left ( \overrightarrow{s} \right )
= 
\left | \overrightarrow{s} \right | ^{2}
= 
\left ( U \overrightarrow{p} \right ) ^{T}
\cdot
\left ( U \overrightarrow{p} \right )
= 
\overrightarrow{p}^{T} \overrightarrow{p}
= 
\sum_{1}^{N} p_{k}^{2}
$$

$$
\overrightarrow{s_{in}}
\left ( \sum_{1}^{N} p_{k} \overrightarrow{u_{k}} \right )
\to H \to
\overrightarrow{s_{out}}
\left ( \sum_{1}^{N} p_{k}^{'} \overrightarrow{u_{k}} \right )
$$

$$
\overrightarrow{s_{in}}
\left ( \sum_{1}^{N} p_{k} \overrightarrow{u_{k}} \right )
\to H \left ( filter \right ) \to
\overrightarrow{s_{out}}
\left ( \sum_{1}^{N}
h \left ( \lambda_{k} \right ) p_{k} \overrightarrow{u_{k}} \right )
$$

$$
\overrightarrow{s_{out}}
= 
H \overrightarrow{s_{in}}
= 
\sum_{1}^{N}
h \left ( \lambda_{k} \right ) p_{k} \overrightarrow{u_{k}}
$$

$$
= 
\begin{bmatrix}
	u_{1} & u_{2} & ... & u_{n}
\end{bmatrix}
\begin{bmatrix}
	h \left ( \lambda_{1} \right ) p_{1} \\
	h \left ( \lambda_{2} \right ) p_{2} \\
	... \\
	h \left ( \lambda_{n} \right ) p_{n}
\end{bmatrix}
$$

$$
= 
U
\begin{bmatrix}
	h \left ( \lambda_{1} \right ) &  &  & \\
	&  h \left ( \lambda_{2} \right ) &  & \\
	&  &  ... & \\
	&  &  & h \left ( \lambda_{n} \right )
\end{bmatrix}
\begin{bmatrix}
	p_{1} \\
	p_{2} \\
	... \\
	p_{n}
\end{bmatrix}
$$

$$
= 
U
\begin{bmatrix}
	h \left ( \lambda_{1} \right ) &  &  & \\
	&  h \left ( \lambda_{2} \right ) &  & \\
	&  &  ... & \\
	&  &  & h \left ( \lambda_{n} \right )
\end{bmatrix}
U^{T} \overrightarrow{s_{in}}
$$

$$
H = 
U
\begin{bmatrix}
	h \left ( \lambda_{1} \right ) &  &  & \\
	&  h \left ( \lambda_{2} \right ) &  & \\
	&  &  ... & \\
	&  &  & h \left ( \lambda_{n} \right )
\end{bmatrix}
U^{T}
= 
U \Lambda_{h} U^{T}
$$

$$
\Lambda_{h} = 
\lim_{K \to \infty} \sum_{0}^{K} h_{k} \Lambda^{k}
$$

$$ K \ll N $$

$$
H = U
\left (
h_{0} \Lambda^{0} +
h_{1} \Lambda^{1} +
h_{2} \Lambda^{2} +
... +
h_{K} \Lambda^{K}
\right )
U^{T}
$$

$$
= 
U \left ( h_{0} \Lambda^{0} \right ) U^{T} +
U \left ( h_{1} \Lambda^{1} \right ) U^{T} +
U \left ( h_{2} \Lambda^{2} \right ) U^{T} +
... +
U \left ( h_{K} \Lambda^{K} \right ) U^{T}
$$

$$
= 
h_{0} L^{0} +
h_{1} L^{1} +
h_{2} L^{2} +
... +
h_{K} L^{K}
= 
\sum_{0}^{K} h_{k} L^{k}
$$

$$
K = 1
$$
$$
H = 
h_{0} L^{0} +
h_{1} L^{1}
$$
\end{abstract}

\section{}

\end{document}
